yalla/mll_def.v
@@ -211,7 +211,7 @@ Ltac no_selfform := try (
 
 (** * MLL Proofs *)
 Inductive ll : list formula -> Type :=
-| ax_r : forall X, ll (covar X :: var X :: nil)
+| ax_r : forall X, ll [:: covar X; var X]
 | ex_r : forall l1 l2, ll l1 -> Permutation_Type l1 l2 -> ll l2
 | tens_r : forall A B l1 l2, ll (A :: l1) -> ll (B :: l2) -> ll (tens A B :: l2 ++ l1)
 | parr_r : forall A B l, ll (A :: B :: l) -> ll (parr A B :: l)
@@ -236,7 +236,7 @@ Lemma psize_rew l l' (pi : ll l) (Heq : l = l') : psize (rew Heq in pi) = psize 
 Proof. now subst. Qed.
 
 (** ** Axiom expansion *)
-Definition ax_exp A : ll (dual A :: A :: nil).
+Definition ax_exp A : ll [:: dual A; A].
 Proof.
   induction A as [ | | A ? B ? | A ? B ?]; cbn.
   - apply ax_r.
